\begin{proof}[Proof of Theorem \ref{the:min}.]
\textbf{Zrob tak zeby sie proof nie powtarzal 2x w naglowku w tym i innych twierdzeniach w appendixie}
Let $X=\{ \x_1, \ldots, \x_n \}$.
We write 
\begin{equation*}
\z_i= W(\x_i-m), \quad \z_{ij}= \w_j^T(\x_i-m),
\end{equation*}
for observation $i$, where $i=1,\ldots,n$ and coordinates $j=1,\ldots,d$.

Let us consider the likelihood function, i.e. 
$$
\begin{array}{l}
L(X;\m,W,\sigma,\tau) = \prod\limits_{i=1}^{n} SN_{d}N_{D-d}(\x_i; \m,W, \sigma^2,\tau^2) \\[6pt] 
=\prod\limits_{i=1}^{n} | \det(W)|  \prod\limits_{j=1}^{d} SN(  \w_j^T (\x_i - \m) ; 0 , \sigma_j^2, \tau_j^2) \cdot %\\[6pt]
\prod\limits_{j=d+1}^{D} N(  \w_j^T (\x_i - \m) ; 0 , \sigma_j^2) =\\[6pt]
\Big( c_1|\det(W)| \Big)^{n} 
\Big( \prod\limits_{j=1}^{d} \sigma_j(1+\tau_j) \Big)^{-n} %\cdot \\[6pt]
\prod\limits_{i=1}^{n} %\\[6pt]
\prod\limits_{j=1}^{d} \exp \Big[ -\frac{1}{2\sigma_j^2}z_{ij}^2 (\1_{ \{ z_{ij} \leq 0 \} } + %\\[6pt]
\tau_{j}^{-2} \1_{ \{ z_{ij} > 0 \} }) \Big] \\[6pt]
\Big( \prod\limits_{j=d+1}^{D} \sigma_j \Big)^{-n} \prod\limits_{i=1}^{n}\prod\limits_{j=d+1}^{D} \exp \Big[ -\frac{1}{2\sigma_j^2}z_{ij}^2 \Big],
\end{array}
$$
%$$
%\begin{array}{l}
%= \prod\limits_{i=1}^{n} GSN_d(\x_i ; \m,V,\sigma,\tau)
%= \prod\limits_{i=1}^{n} \frac{1}{| \det( V)|}  \prod\limits_{j=1}^{d} SN(  \v^{-1}_j \x_i ; \v^{-1}_j \m , \sigma_j^2, \tau_j^2)=
%\\[1ex]
%\left(\frac{c_1}{|\det(V)|}\right)^{n} \left( \prod\limits_{j=1}^{d} \sigma_j(1+\tau_j) \right)^{-n} \left( \prod\limits_{i=1}^{n} \prod\limits_{j=1}^{d} \exp[-\frac{1}{2\sigma_j^2}z_{ij}^2 (\1_{ \{ z_{ij} \leq 0 \} } + \tau_{j}^{-2} \1_{ \{ z_{ij} > 0 \} })]\right)
%\end{array}
%$$
where 
$
c_1= \left( \sqrt{\tfrac{2}{\pi}} \right)^{d} \cdot \left( \tfrac{1}{ \sqrt{2\pi} } \right)^{D-d}.
$
Now we take the log-likelihood function, i.e. 
$$
\begin{array}{l}
\ln(L(X;\m,W,\sigma,\tau)) = \ln \bigg( \Big( c_1|\det(W)| \Big)^{n} \Big( \prod\limits_{j=1}^{d} \sigma_j(1+\tau_j) \Big)^{-n} \Big( \prod\limits_{j=d+1}^{D} \sigma_j \Big)^{-n}  \bigg) + \\[6pt]
 \sum\limits_{i=1}^{n} \sum\limits_{j=1}^{d} \Big[ -\frac{1}{2\sigma_j^2}z_{ij}^2 (\1_{ \{ z_{ij} \leq 0 \} } + \tau_{j}^{-2} \1_{ \{ z_{ij} > 0 \} })\Big] +  %\\[6pt]
 \sum\limits_{i=1}^{n} \sum\limits_{j=d+1}^{D} \Big[ -\frac{1}{2\sigma_j^2}z_{ij}^2 \Big]  \\[6pt]
= \ln \bigg( \Big( c_1|\det(W)| \Big)^{n} \Big( \prod\limits_{j=1}^{d} (1+\tau_j) \Big)^{-n} \Big( \prod\limits_{j=1}^{D} \sigma_j \Big)^{-n} \bigg)  - \\[6pt]
  \frac{1}{2} \sum\limits_{j=1}^{d} \Big( \sigma_j^{-2} \sum\limits_{i \in I_{j}}    z_{ij}^2   + \frac{\sigma_j^{-2}}{\tau_{j}^{2} }  \sum\limits_{i \in I_{j}^{c}}   z_{ij}^2  \Big) -  %\\[6pt]
  \frac{1}{2} \sum\limits_{j=d+1}^{D} \sigma_j^{-2} \Big( \sum\limits_{i \in I_{j}}    z_{ij}^2   +  \sum\limits_{i \in I_{j}^{c}}   z_{ij}^2  \Big) \\[6pt]
= \ln \bigg( \Big( c_1|\det(W)| \Big)^{n} \Big( \prod\limits_{j=1}^{d} (1+\tau_j) \Big)^{-n} \Big( \prod\limits_{j=1}^{D} \sigma_j \Big)^{-n} \bigg) - \\[6pt]
 \sum\limits_{j=1}^{d} \frac{1}{2\sigma_j^{2}} \Big(  s_{1j}  + \frac{1}{\tau_{j}^{2} }  s_{2j}  \Big) - \sum\limits_{j=d+1}^{D} \frac{1}{2\sigma_j^{2}} \Big(  s_{1j}  + s_{2j}  \Big).
\end{array}
$$

We fix  $\m$, $W$ and maximize the log-likelihood function over $\tau$ and $\sigma$.
In such a case \textbf{zamiast In such a case uzyj Consequently} we have to \textbf{zamiast we have to uzyj we need to} solve the following system of equations
$$
\begin{array}{l}
\frac{\partial  \ln ( L(X;\m,W,\sigma,\tau) ) }{\partial \sigma_j} =0, \qquad %\\[6pt] & \mbox{ for }  & j=1,\ldots,d,
 \frac{\partial  \ln ( L(X;\m,W,\sigma,\tau) ) }{\partial \tau_j} =0 , %& \mbox{ for }  & j=1,\ldots,d.
\end{array}
$$
for  $ j=1,\ldots,D$. Hence \textbf{It follows that zamiast Hence}
$$
\begin{array}{l}
-\frac{n}{\sigma_j} +  \sigma_j^{-3} (s_{1j} + \tau_j^{-2} s_{2j} ) = 0, \mbox{ for }  j=1,\ldots,d,\\[6pt]
 -\frac{n}{\sigma_j} +  \sigma_j^{-3} (s_{1j} + s_{2j} ) =0, \mbox{ for } j>d, \\[6pt] %
- \frac{n}{1+\tau_j} + \frac{s_{2j}}{\tau_j^{3}\sigma_j^{2}} =0 , \mbox{ for } j=1,\ldots,d.
\end{array}
$$
By simple calculations we obtain the expressions for the estimators in \ref{eq:est}.
%\begin{align*}
%$$
%\hat{\sigma}_j^2(\m,W) = 
%\tfrac{1}{n} s_{1j}^{2/3} g_{j}(\m,W), \qquad
%\hat{\tau}_{j}(\m,W) = \bigg( \frac{s_{2j}}{s_{1j}} \bigg)^{1/3}.
%$$
%\end{align*}
Substituting it into the log-likelihood function,
%and taking $e^{\ln \hat{L}(\m,W)}$
we get %$$
$$
\begin{array}{l}
\hat{L}(\m,W) = \bigg( \frac{2}{\pi} \bigg)^{\frac{dn}{2}}  \bigg( \frac{1}{2\pi} \bigg)^{\frac{(D-d)n}{2}} \!\!\!\!\! |\det(W)|^{n} \Big( \prod\limits_{j=1}^{d} \frac{1}{\sqrt{n}} g_j(\m,W)^{\frac{3}{2}} \Big)^{-n} \!\!\!\!\!
e^{-\frac{dn}{2}} \Big( \prod\limits_{j=d+1}^{D} (\frac{s_{1j} + s_{2j}}{n})^{\frac{1}{2}} \Big)^{-n} \!\!\!\!\! = \\[6pt]
\frac{ 2^{(d-D/2)n} n^{dn/2} }{(\pi e)^{Dn/2}} \cdot %\\[6pt]
\Big( \frac{1}{|\det(W)|^{\frac{2}{3}}} \prod\limits_{j=1}^{d} g_j(\m,W) \Big)^{-\frac{3n}{2}} \Big( \prod\limits_{j=d+1}^{D} \frac{(s_{1j} + s_{2j})}{n} \Big)^{-\frac{n}{2}} 
\end{array}
$$
%= \bigg( \frac{2n}{\pi e} \bigg)^{\frac{dn}{2}} =
\end{proof}
